Bdd/Prime.lean
@@ -2,26 +2,28 @@ import Bdd.Basic
 
 namespace Prime
 
-def prime_node (p : Nat): Node n m → Node (n + p) m
-  | ⟨var, low, high⟩ => ⟨⟨var.1 + p, (add_lt_add_iff_right p).mpr (Fin.is_lt var)⟩, low, high⟩
+def relabel_node {f : Nat → Nat} (hf : ∀ i : Fin n, f i < f n) : Node n m → Node (f n) m
+  | ⟨var, low, high⟩ => ⟨⟨f var.1, hf _⟩, low, high⟩
 
-def prime_heap (p : Nat): Vector (Node n m) m → Vector (Node (n + p) m) m := Vector.map (prime_node p)
+def relabel_heap {f : Nat → Nat} (hf : ∀ i : Fin n, f i < f n) :
+    Vector (Node n m) m → Vector (Node (f n) m) m := Vector.map (relabel_node hf)
 
-def prime (p : Nat) : Bdd n m → Bdd (n + p) m
-  | ⟨heap, root⟩ => ⟨prime_heap p heap, root⟩
+def relabel {f : Nat → Nat} (hf : ∀ i : Fin n, f i < f n) : Bdd n m → Bdd (f n) m
+  | ⟨heap, root⟩ => ⟨relabel_heap hf heap, root⟩
 
-lemma prime_edge_iff {B : Bdd n m} {x y : Pointer m} : Edge B.heap x y ↔ Edge (prime p B).heap x y := by
+lemma relabel_edge_iff {B : Bdd n m} {x y : Pointer m} {f : Nat → Nat} {hf : ∀ i : Fin n, f i < f n} :
+    Edge B.heap x y ↔ Edge (relabel hf B).heap x y := by
   constructor
   · intro e
     cases e with
-    | low  _ => left;  simpa [prime, prime_heap]
-    | high _ => right; simpa [prime, prime_heap]
+    | low  _ => left;  simpa [relabel, relabel_heap]
+    | high _ => right; simpa [relabel, relabel_heap]
   · intro e
     cases e with
-    | low  _ => left;  simp_all [prime, prime_heap, prime_node]; assumption
-    | high _ => right; simp_all [prime, prime_heap, prime_node]; assumption
+    | low  _ => left;  simp_all [relabel, relabel_heap, relabel_node]; assumption
+    | high _ => right; simp_all [relabel, relabel_heap, relabel_node]; assumption
 
-lemma prime_reachable_iff {B : Bdd n m} : Pointer.Reachable B.heap B.root x ↔ Pointer.Reachable (prime p B).heap (prime p B).root x := by
+lemma relabel_reachable_iff {B : Bdd n m} : Pointer.Reachable B.heap B.root x ↔ Pointer.Reachable (relabel h B).heap (relabel h B).root x := by
   constructor
   · intro r
     induction r with
@@ -29,78 +31,84 @@ lemma prime_reachable_iff {B : Bdd n m} : Pointer.Reachable B.heap B.root x ↔ 
     | tail _ e ih =>
       right
       · exact ih
-      · exact (prime_edge_iff.mp e)
+      · exact (relabel_edge_iff.mp e)
   · intro r
     induction r with
     | refl => left
     | tail _ e ih =>
       right
       · exact ih
-      · exact (prime_edge_iff.mpr e)
+      · exact (relabel_edge_iff.mpr e)
 
-lemma prime_mayPrecede_iff {B : Bdd n m} {x y : Pointer m}: Pointer.MayPrecede B.heap x y ↔ Pointer.MayPrecede (prime p B).heap x y := by
-  constructor
-  · intro h
-    cases x with
-    | terminal _ => absurd h; exact Pointer.not_terminal_MayPrecede
-    | node _ =>
-      cases y with
-      | terminal _ => apply Pointer.MayPrecede_node_terminal
-      | node _ =>
-        simp only [Pointer.MayPrecede, prime, prime_heap, Pointer.toVar] at h
-        simp only [Nat.succ_eq_add_one, Fin.getElem_fin, Fin.coe_eq_castSucc, Fin.castSucc_lt_castSucc_iff] at h
-        simp only [Pointer.MayPrecede, prime, prime_heap, Pointer.toVar]
-        simp only [Nat.succ_eq_add_one, Fin.getElem_fin, Vector.getElem_map, Fin.coe_eq_castSucc, Fin.castSucc_lt_castSucc_iff]
-        simp only [prime_node]
-        simp only [Fin.eta, Fin.mk_lt_mk, add_lt_add_iff_right, Fin.val_fin_lt]
-        exact h
-  · intro h
-    cases x with
-    | terminal _ => absurd h; exact Pointer.not_terminal_MayPrecede
-    | node _ =>
-      cases y with
-      | terminal _ => apply Pointer.MayPrecede_node_terminal
-      | node _ =>
-        simp only [Pointer.MayPrecede, prime, prime_heap, Pointer.toVar]
-        simp only [Nat.succ_eq_add_one, Fin.getElem_fin, Fin.coe_eq_castSucc, Fin.castSucc_lt_castSucc_iff]
-        simp only [Pointer.MayPrecede, prime, prime_heap, Pointer.toVar] at h
-        simp only [Nat.succ_eq_add_one, Fin.getElem_fin, Vector.getElem_map, Fin.coe_eq_castSucc, Fin.castSucc_lt_castSucc_iff] at h
-        simp only [prime_node] at h
-        simp only [Fin.eta, Fin.mk_lt_mk, add_lt_add_iff_right, Fin.val_fin_lt] at h
-        exact h
-
-lemma prime_relevantMayPrecede {B : Bdd n m} {x y : Pointer m} {hx : Pointer.Reachable (prime p B).heap (prime p B).root x} {hy : Pointer.Reachable (prime p B).heap (prime p B).root y} :
-    B.RelevantMayPrecede ⟨x, prime_reachable_iff.mpr hx⟩ ⟨y, prime_reachable_iff.mpr hy⟩ → (prime p B).RelevantMayPrecede ⟨x, hx⟩ ⟨y, hy⟩ := prime_mayPrecede_iff.mp
-
-lemma prime_relevantEdge {B : Bdd n m} {x y : Pointer m} {hx : Pointer.Reachable (prime p B).heap (prime p B).root x} {hy : Pointer.Reachable (prime p B).heap (prime p B).root y} :
-    (prime p B).RelevantEdge ⟨x, hx⟩ ⟨y, hy⟩ → B.RelevantEdge ⟨x, prime_reachable_iff.mpr hx⟩ ⟨y, prime_reachable_iff.mpr hy⟩ := by
+lemma relabel_relevantMayPrecede {B : Bdd n m} {f : Nat → Nat} {hf : ∀ i : Fin n, f i < f n}
+    {hu : ∀ i i' : Fin n, i < i' → B.usesVar i → B.usesVar i' → f i < f i'}
+    {x y : Pointer m}
+    {hx : Pointer.Reachable (relabel hf B).heap (relabel hf B).root x}
+    {hy : Pointer.Reachable (relabel hf B).heap (relabel hf B).root y} :
+    B.RelevantMayPrecede ⟨x, relabel_reachable_iff.mpr hx⟩ ⟨y, relabel_reachable_iff.mpr hy⟩ → (relabel hf B).RelevantMayPrecede ⟨x, hx⟩ ⟨y, hy⟩ := by
   intro h
-  simp_all only [Bdd.RelevantEdge, prime, prime_heap]
+  simp only [Bdd.RelevantMayPrecede] at h
+  simp only [Bdd.RelevantMayPrecede]
+  cases x with
+  | terminal _ => absurd h; exact Pointer.not_terminal_MayPrecede
+  | node j =>
+    cases y with
+    | terminal _ => apply Pointer.MayPrecede_node_terminal
+    | node j' =>
+      simp only [Pointer.MayPrecede, relabel, relabel_heap, Pointer.toVar] at h
+      simp only [Nat.succ_eq_add_one, Fin.getElem_fin, Fin.coe_eq_castSucc, Fin.castSucc_lt_castSucc_iff] at h
+      simp only [Pointer.MayPrecede, relabel, relabel_heap, Pointer.toVar]
+      simp only [Nat.succ_eq_add_one, Fin.getElem_fin, Vector.getElem_map, Fin.coe_eq_castSucc, Fin.castSucc_lt_castSucc_iff]
+      simp only [relabel_node]
+      simp only [Fin.eta, Fin.mk_lt_mk, add_lt_add_iff_right, Fin.val_fin_lt]
+      apply hu
+      · exact h
+      · use j
+        constructor
+        · exact relabel_reachable_iff.mpr hx
+        · rfl
+      · use j'
+        constructor
+        · exact relabel_reachable_iff.mpr hy
+        · rfl
+
+lemma relabel_relevantEdge {B : Bdd n m} {f : Nat → Nat} {hf : ∀ i : Fin n, f i < f n}
+    {x y : Pointer m}
+    {hx : Pointer.Reachable (relabel hf B).heap (relabel hf B).root x}
+    {hy : Pointer.Reachable (relabel hf B).heap (relabel hf B).root y} :
+    (relabel hf B).RelevantEdge ⟨x, hx⟩ ⟨y, hy⟩ → B.RelevantEdge ⟨x, relabel_reachable_iff.mpr hx⟩ ⟨y, relabel_reachable_iff.mpr hy⟩ := by
+  intro h
+  simp_all only [Bdd.RelevantEdge, relabel, relabel_heap]
   cases h with
   | low _ =>
     left
-    simp_all [prime_node]
+    simp_all [relabel_node]
     assumption
   | high _ =>
     right
-    simp_all [prime_node]
+    simp_all [relabel_node]
     assumption
 
-lemma prime_preserves_ordered : Bdd.Ordered B → Bdd.Ordered (prime p B) := by
-  intro ho
+lemma relabel_preserves_ordered {B : Bdd n m} {f : Nat → Nat} {hf : ∀ i : Fin n, f i < f n} :
+    (∀ i i' : Fin n, i < i' → B.usesVar i → B.usesVar i' → f i < f i') → Bdd.Ordered B → Bdd.Ordered (relabel hf B) := by
+  intro hu ho
   rintro _ _ hxy
-  apply prime_relevantMayPrecede
+  apply relabel_relevantMayPrecede
+  exact hu
   apply ho
-  exact prime_relevantEdge hxy
+  exact relabel_relevantEdge hxy
 
-def oprime p : OBdd n m → OBdd (n + p) m
-  | O => ⟨prime p O.1, prime_preserves_ordered O.2⟩
+def orelabel (O : OBdd n m) {f : Nat → Nat} (hf : ∀ i : Fin n, f i < f n)
+    (hu : ∀ i i' : Fin n, i < i' → O.1.usesVar i → O.1.usesVar i' → f i < f i') : OBdd (f n) m :=
+    ⟨(relabel hf O.1), relabel_preserves_ordered hu O.2⟩
 
-lemma oprime_low {n m j p} {O : OBdd n m} {h : O.1.root = .node j} : (OBdd.low (oprime p O) h) = oprime p (O.low h) := by
+lemma orelabel_low {O : OBdd n m} {h : O.1.root = .node j} {f : Nat → Nat} (hf : ∀ i : Fin n, f i < f n)
+    (hu : ∀ i i' : Fin n, i < i' → O.1.usesVar i → O.1.usesVar i' → f i < f i') :
+    (OBdd.low (orelabel O hf hu) h) = orelabel (O.low h) hf (fun i i' hii' hi hi' ↦ hu i i' hii' (OBdd.usesVar_of_low_usesVar hi) (OBdd.usesVar_of_low_usesVar hi')) := by
   rcases O with ⟨B, o⟩
   simp only [OBdd.low]
   congr
-  simp only [oprime, prime, prime_heap, Bdd.low_heap_eq_heap]
+  simp only [orelabel, relabel, relabel_heap, Bdd.low_heap_eq_heap]
   simp only at h
   simp_rw [h]
   simp only [Bdd.low]
@@ -108,11 +116,13 @@ lemma oprime_low {n m j p} {O : OBdd n m} {h : O.1.root = .node j} : (OBdd.low (
   simp_all only [Fin.getElem_fin, Vector.getElem_map]
   rfl
 
-lemma oprime_high {n m j p} {O : OBdd n m} {h : O.1.root = .node j} : (OBdd.high (oprime p O) h) = oprime p (O.high h) := by
+lemma orelabel_high {O : OBdd n m} {h : O.1.root = .node j} {f : Nat → Nat} (hf : ∀ i : Fin n, f i < f n)
+    (hu : ∀ i i' : Fin n, i < i' → O.1.usesVar i → O.1.usesVar i' → f i < f i') :
+    (OBdd.high (orelabel O hf hu) h) = orelabel (O.high h) hf (fun i i' hii' hi hi' ↦ hu i i' hii' (OBdd.usesVar_of_high_usesVar hi) (OBdd.usesVar_of_high_usesVar hi')) := by
   rcases O with ⟨B, o⟩
   simp only [OBdd.high]
   congr
-  simp only [oprime, prime, prime_heap, Bdd.high_heap_eq_heap]
+  simp only [orelabel, relabel, relabel_heap, Bdd.high_heap_eq_heap]
   simp only at h
   simp_rw [h]
   simp only [Bdd.high]
@@ -120,108 +130,57 @@ lemma oprime_high {n m j p} {O : OBdd n m} {h : O.1.root = .node j} : (OBdd.high
   simp_all only [Fin.getElem_fin, Vector.getElem_map]
   rfl
 
-lemma bprime_low {n m j p} {B : Bdd n m} {o : Bdd.Ordered B} {h : B.root = .node j} : (OBdd.low ⟨prime p B, prime_preserves_ordered o⟩ h) = ⟨prime p (OBdd.low ⟨B, o⟩ h).1, prime_preserves_ordered (OBdd.low ⟨B, o⟩ h).2⟩ := by
-  simp only [OBdd.low]
-  congr
-  simp only [prime, prime_heap, Bdd.low_heap_eq_heap]
-  simp_rw [h]
-  simp only [Bdd.low]
-  congr 1
-  simp_all only [Fin.getElem_fin, Vector.getElem_map]
-  rfl
+lemma brelabel_low {B : Bdd n m} {o : Bdd.Ordered B} {h : B.root = .node j} {f : Nat → Nat} (hf : ∀ i : Fin n, f i < f n)
+    (hu : ∀ i i' : Fin n, i < i' → B.usesVar i → B.usesVar i' → f i < f i') :
+    (OBdd.low ⟨relabel hf B, relabel_preserves_ordered hu o⟩ h) =
+      ⟨relabel hf (OBdd.low ⟨B, o⟩ h).1, relabel_preserves_ordered (fun i i' hii' hi hi' ↦ hu i i' hii' (OBdd.usesVar_of_low_usesVar hi) (OBdd.usesVar_of_low_usesVar hi')) (OBdd.low ⟨B, o⟩ h).2⟩ := by
+  exact orelabel_low (O := ⟨B, o⟩) hf hu
 
-lemma bprime_high {n m j p} {B : Bdd n m} {o : Bdd.Ordered B} {h : B.root = .node j} : (OBdd.high ⟨prime p B, prime_preserves_ordered o⟩ h) = ⟨prime p (OBdd.high ⟨B, o⟩ h).1, prime_preserves_ordered (OBdd.high ⟨B, o⟩ h).2⟩ := by
-  simp only [OBdd.high]
-  congr
-  simp only [prime, prime_heap, Bdd.high_heap_eq_heap]
-  simp_rw [h]
-  simp only [Bdd.high]
-  congr 1
-  simp_all only [Fin.getElem_fin, Vector.getElem_map]
-  rfl
+lemma brelabel_high {B : Bdd n m} {o : Bdd.Ordered B} {h : B.root = .node j} {f : Nat → Nat} (hf : ∀ i : Fin n, f i < f n)
+    (hu : ∀ i i' : Fin n, i < i' → B.usesVar i → B.usesVar i' → f i < f i') :
+    (OBdd.high ⟨relabel hf B, relabel_preserves_ordered hu o⟩ h) =
+      ⟨relabel hf (OBdd.high ⟨B, o⟩ h).1, relabel_preserves_ordered (fun i i' hii' hi hi' ↦ hu i i' hii' (OBdd.usesVar_of_high_usesVar hi) (OBdd.usesVar_of_high_usesVar hi')) (OBdd.high ⟨B, o⟩ h).2⟩ := by
+  exact orelabel_high (O := ⟨B, o⟩) hf hu
 
-lemma prime_low {n m j p} {O : OBdd n m} {h : O.1.root = .node j} : (OBdd.low ⟨prime p O.1, prime_preserves_ordered O.2⟩ h) = ⟨prime p (O.low h).1, prime_preserves_ordered (O.low h).2⟩ := by
-  simp only [OBdd.low]
-  congr
-  simp only [prime, prime_heap, Bdd.low_heap_eq_heap]
-  simp_rw [h]
-  simp only [Bdd.low]
-  congr 1
-  simp_all only [Fin.getElem_fin, Vector.getElem_map]
-  rfl
-
-lemma prime_high {n m j p} {O : OBdd n m} {h : O.1.root = .node j} : (OBdd.high ⟨prime p O.1, prime_preserves_ordered O.2⟩ h) = ⟨prime p (O.high h).1, prime_preserves_ordered (O.high h).2⟩ := by
-  simp only [OBdd.high]
-  congr
-  simp only [prime, prime_heap, Bdd.high_heap_eq_heap]
-  simp_rw [h]
-  simp only [Bdd.high]
-  congr 1
-  simp_all only [Fin.getElem_fin, Vector.getElem_map]
-  rfl
-
-theorem oprime_evaluate (O : OBdd n m) : OBdd.evaluate (oprime p O) I = O.evaluate (Vector.cast (show n + p - p = n from Eq.symm (Nat.eq_sub_of_add_eq rfl)) (I.drop p)) := by
-  simp only [oprime]
+theorem orelabel_evaluate (O : OBdd n m) {f : Nat → Nat} {hf : ∀ i : Fin n, f i < f n}
+    {hu : ∀ i i' : Fin n, i < i' → O.1.usesVar i → O.1.usesVar i' → f i < f i'} {I : Vector Bool (f n)} :
+    OBdd.evaluate (orelabel O hf hu) I = O.evaluate (Vector.ofFn (fun i ↦ I[f i]'(hf i))) := by
+  simp only [orelabel]
   cases O_root_def : O.1.root with
   | terminal _ =>
-    simp only [prime]
+    simp only [relabel]
     rw [OBdd.evaluate_terminal' O_root_def]
     simp_rw [O_root_def]
     rw [OBdd.evaluate_terminal]
     simp
   | node j =>
     rw [OBdd.evaluate_node'' O_root_def]
-    have that : (⟨(prime p O.1), prime_preserves_ordered O.2⟩ : OBdd _ _).1.root = Pointer.node j := O_root_def
+    have that : (⟨(relabel hf O.1), relabel_preserves_ordered hu O.2⟩ : OBdd _ _).1.root = Pointer.node j := O_root_def
     rw [OBdd.evaluate_node'' that]
     simp only
     congr 1
     · simp only [eq_iff_iff, Bool.coe_iff_coe]
-      simp only [prime, prime_heap, Fin.getElem_fin, Vector.getElem_map, prime_node]
+      simp only [relabel, relabel_heap, Fin.getElem_fin, Vector.getElem_map, relabel_node]
       simp only [Fin.eta]
-      rw [Vector.getElem_cast]
-      symm
-      simp_rw [add_comm]
-      apply Vector.getElem_drop
-    · have := oprime_evaluate (O.high O_root_def) (I := I)
-      rw [← this]
-      rw [← oprime_high]
+      simp_all only [Vector.getElem_ofFn]
       rfl
-    · have := oprime_evaluate (O.low O_root_def) (I := I)
+    · have := orelabel_evaluate
+        (hu := (fun i i' hii' hi hi' ↦ hu i i' hii' (OBdd.usesVar_of_high_usesVar hi) (OBdd.usesVar_of_high_usesVar hi')))
+        (hf := hf)
+        (O.high O_root_def) (I := I)
       rw [← this]
-      rw [← oprime_low]
+      rw [← orelabel_high hf hu]
+      rfl
+    · have := orelabel_evaluate
+        (hu := (fun i i' hii' hi hi' ↦ hu i i' hii' (OBdd.usesVar_of_low_usesVar hi) (OBdd.usesVar_of_low_usesVar hi')))
+        (hf := hf)
+        (O.low O_root_def) (I := I)
+      rw [← this]
+      rw [← orelabel_low hf hu]
       rfl
 termination_by O
 
-theorem prime_evaluate (O : OBdd n m) : OBdd.evaluate ⟨prime p O.1, prime_preserves_ordered O.2⟩ I = O.evaluate (Vector.cast (show n + p - p = n from Eq.symm (Nat.eq_sub_of_add_eq rfl)) (I.drop p)) := by
-  cases O_root_def : O.1.root with
-  | terminal _ =>
-    simp only [prime]
-    rw [OBdd.evaluate_terminal' O_root_def]
-    simp_rw [O_root_def]
-    rw [OBdd.evaluate_terminal]
-    simp
-  | node j =>
-    rw [OBdd.evaluate_node'' O_root_def]
-    have that : (⟨(prime p O.1), prime_preserves_ordered O.2⟩ : OBdd _ _).1.root = Pointer.node j := O_root_def
-    rw [OBdd.evaluate_node'' that]
-    simp only
-    congr 1
-    · simp only [eq_iff_iff, Bool.coe_iff_coe]
-      simp only [prime, prime_heap, Fin.getElem_fin, Vector.getElem_map, prime_node]
-      simp only [Fin.eta]
-      rw [Vector.getElem_cast]
-      symm
-      simp_rw [add_comm]
-      apply Vector.getElem_drop
-    · have := prime_evaluate (O.high O_root_def) (I := I)
-      rw [← this]
-      rw [← prime_high]
-    · have := prime_evaluate (O.low O_root_def) (I := I)
-      rw [← this]
-      rw [← prime_low]
-termination_by O
-
-lemma prime_preserves_noRedundancy {B : Bdd n m} : B.NoRedundancy → (prime p B).NoRedundancy := by
+lemma relabel_preserves_noRedundancy {B : Bdd n m} : B.NoRedundancy → (relabel hf B).NoRedundancy := by
   rintro hnr ⟨p, hp⟩ contra
   simp only at contra
   cases p_def : p with
@@ -232,430 +191,80 @@ lemma prime_preserves_noRedundancy {B : Bdd n m} : B.NoRedundancy → (prime p B
     rw [p_def] at contra
     cases contra with
     | red red =>
-      simp only [prime, prime_heap, Fin.getElem_fin, prime_node] at red
-      apply hnr ⟨p, prime_reachable_iff.mpr hp⟩
+      simp only [relabel, relabel_heap, Fin.getElem_fin, relabel_node] at red
+      apply hnr ⟨p, relabel_reachable_iff.mpr hp⟩
       simp_rw [p_def]
       constructor
       simp_all only [Vector.getElem_map, Fin.getElem_fin]
-      simp only [prime, prime_heap, Fin.getElem_fin, prime_node] at red
+      simp only [relabel, relabel_heap, Fin.getElem_fin, relabel_node] at red
       exact red
 
-def tprime p : DecisionTree n → DecisionTree (n + p)
+def trelabel {f : Nat → Nat} (hf : ∀ i : Fin n, f i < f n) : DecisionTree n → DecisionTree (f n)
   | .leaf b => .leaf b
-  | .branch i l h => .branch ⟨i.1 + p, by omega⟩ (tprime p l) (tprime p h)
+  | .branch i l h => .branch ⟨f i, hf i⟩ (trelabel hf l) (trelabel hf h)
 
-lemma tprime_injective : Function.Injective (tprime (n := n) p) := by
-  intro x y hxy
-  cases x with
-  | leaf _ =>
-    cases y with
-    | leaf _ => simp only [tprime] at hxy; simp_all
-    | branch _ _ _ => contradiction
-  | branch _ _ _ =>
-    cases y with
-    | leaf _ => contradiction
-    | branch _ _ _ =>
-      simp only [tprime] at hxy
-      injection hxy with a b c
-      rw [tprime_injective b, tprime_injective c]
-      aesop
-
-lemma prime_toTree_tprime' {O : OBdd n m} :
-    OBdd.toTree ⟨prime p O.1, prime_preserves_ordered O.2⟩ = tprime p (OBdd.toTree O) := by
-  cases O_root_def : O.1.root with
-  | terminal _ =>
-    simp only [prime]
-    rw [OBdd.toTree_terminal' O_root_def]
-    simp_rw [O_root_def]
-    rw [OBdd.toTree_terminal]
-    simp [tprime]
-  | node _ =>
-    -- simp only [prime]
-    rw [OBdd.toTree_node O_root_def]
-    rw [OBdd.toTree_node (by trans O.1.root; rfl; exact O_root_def)]
-    simp only [Fin.getElem_fin]
-    congr 1
-    · simp only [prime, prime_heap, Vector.getElem_map, prime_node, Fin.eta, Bdd.Ordered.eq_1, Fin.mk.injEq, Nat.add_right_cancel_iff]
-      rfl
-    · have := prime_toTree_tprime' (O := (O.low O_root_def)) (p := p)
-      rw [← prime_low] at this
-      exact this
-    · have := prime_toTree_tprime' (O := (O.high O_root_def)) (p := p)
-      rw [← prime_high] at this
-      exact this
-termination_by O
-
-lemma prime_toTree_tprime {B : Bdd n m} {o : B.Ordered} :
-    OBdd.toTree ⟨prime p B, prime_preserves_ordered o⟩ = tprime p (OBdd.toTree ⟨B, o⟩) := by
-  let O : OBdd n m := ⟨B, o⟩
-  have : B = O.1 := rfl
-  simp_rw [this]
-  exact prime_toTree_tprime'
-
-lemma oprime_preserves_similarRP {O : OBdd n m} {p q : Pointer m} {hp : Pointer.Reachable (oprime x O).1.heap (oprime x O).1.root p} {hq : Pointer.Reachable (oprime x O).1.heap (oprime x O).1.root q} :
-    (oprime x O).SimilarRP ⟨p, hp⟩ ⟨q, hq⟩ → O.SimilarRP ⟨p, prime_reachable_iff.mpr hp⟩ ⟨q, prime_reachable_iff.mpr hq⟩ := by
-  intro sim
-  simp only [OBdd.SimilarRP, OBdd.Similar, OBdd.HSimilar] at sim
-  simp only [OBdd.SimilarRP, OBdd.Similar, OBdd.HSimilar]
-  cases p with
-  | terminal _ =>
-    cases q with
-    | terminal _ => simp_all
-    | node _ =>
-      simp only [OBdd.toTree_terminal] at sim
-      rw [OBdd.toTree_node rfl] at sim
-      contradiction
-  | node j =>
-    cases q with
-    | terminal _ =>
-      simp only [OBdd.toTree_terminal] at sim
-      rw [OBdd.toTree_node rfl] at sim
-      contradiction
-    | node i =>
-      conv at sim =>
-        lhs
-        rw [OBdd.toTree_node rfl]
-      conv at sim =>
-        rhs
-        rw [OBdd.toTree_node rfl]
-      injection sim with ha hb hc
-      simp only [Fin.getElem_fin] at ha
-      simp only [oprime, prime, prime_heap, Vector.getElem_map, prime_node, Fin.eta, Fin.mk.injEq, Nat.add_right_cancel_iff] at ha
-      conv =>
-        lhs
-        rw [OBdd.toTree_node rfl]
-      conv =>
-        rhs
-        rw [OBdd.toTree_node rfl]
-      congr 1
-      · simp only
-        exact Fin.eq_of_val_eq ha
-      · simp only [oprime] at hb
-        simp only [prime] at hb
-        simp_rw [← prime.eq_1] at hb
-        conv at hb =>
-          lhs
-          rw [bprime_low (h := rfl) (o := Bdd.ordered_of_reachable (prime_reachable_iff.mpr hp))]
-        conv at hb =>
-          rhs
-          rw [bprime_low (h := rfl) (o := Bdd.ordered_of_reachable (prime_reachable_iff.mpr hq))]
-        simp only [OBdd.low] at hb
-        simp only [OBdd.low]
-        conv at hb =>
-          lhs
-          rw [prime_toTree_tprime (o := (by apply Bdd.low_ordered; exact Bdd.ordered_of_reachable (prime_reachable_iff.mpr hp)))]
-        conv at hb =>
-          rhs
-          rw [prime_toTree_tprime (o := (by apply Bdd.low_ordered; exact Bdd.ordered_of_reachable (prime_reachable_iff.mpr hq)))]
-        rw [tprime_injective hb]
-      · simp only [oprime] at hc
-        simp only [prime] at hc
-        simp_rw [← prime.eq_1] at hc
-        conv at hc =>
-          lhs
-          rw [bprime_high (h := rfl) (o := Bdd.ordered_of_reachable (prime_reachable_iff.mpr hp))]
-        conv at hc =>
-          rhs
-          rw [bprime_high (h := rfl) (o := Bdd.ordered_of_reachable (prime_reachable_iff.mpr hq))]
-        simp only [OBdd.high] at hc
-        simp only [OBdd.high]
-        conv at hc =>
-          lhs
-          rw [prime_toTree_tprime (o := (by apply Bdd.high_ordered; exact Bdd.ordered_of_reachable (prime_reachable_iff.mpr hp)))]
-        conv at hc =>
-          rhs
-          rw [prime_toTree_tprime (o := (by apply Bdd.high_ordered; exact Bdd.ordered_of_reachable (prime_reachable_iff.mpr hq)))]
-        rw [tprime_injective hc]
-
-lemma oprime_reduced {O : OBdd n m} : O.Reduced → (oprime p O).Reduced := by
-  rintro ⟨r1, r2⟩
-  constructor
-  · exact prime_preserves_noRedundancy r1
-  · rintro _ _ sim; exact r2 (oprime_preserves_similarRP sim)
-
-def unprime_node (p : Fin n) : Node n m → Node (n - p) m
-  | ⟨var, low, high⟩ => ⟨⟨var.1 - p.1, by omega⟩, low, high⟩
-
-def unprime_heap (p : Fin n) : Vector (Node n m) m → Vector (Node (n - p) m) m := Vector.map (unprime_node p)
-
-def unprime (p : Fin n) : Bdd n m → Bdd (n - p) m
-  | ⟨heap, root⟩ => ⟨unprime_heap p heap, root⟩
-
-lemma unprime_edge_iff {B : Bdd n m} {x y : Pointer m} : Edge B.heap x y ↔ Edge (unprime p B).heap x y := by
-  constructor
-  · intro e
-    cases e with
-    | low  _ => left;  simpa [unprime, unprime_heap]
-    | high _ => right; simpa [unprime, unprime_heap]
-  · intro e
-    cases e with
-    | low  _ => left;  simp_all [unprime, unprime_heap]; assumption
-    | high _ => right; simp_all [unprime, unprime_heap]; assumption
-
-lemma unprime_reachable_iff {B : Bdd n m} : Pointer.Reachable B.heap B.root x ↔ Pointer.Reachable (unprime p B).heap (unprime p B).root x := by
-  constructor
-  · intro r
-    induction r with
-    | refl => left
-    | tail _ e ih =>
-      right
-      · exact ih
-      · exact (unprime_edge_iff.mp e)
-  · intro r
-    induction r with
-    | refl => left
-    | tail _ e ih =>
-      right
-      · exact ih
-      · exact (unprime_edge_iff.mpr e)
-
-lemma unprime_mayPrecede {B : Bdd n m} {x y : Pointer m} {p : Fin n} : p ≤ x.toVar B.heap → Pointer.MayPrecede B.heap x y → Pointer.MayPrecede (unprime p B).heap x y := by
-  intro hp h
-  cases x with
-  | terminal _ => absurd h; exact Pointer.not_terminal_MayPrecede
-  | node _ =>
-    cases y with
-    | terminal _ => apply Pointer.MayPrecede_node_terminal
-    | node _ =>
-      simp only [Pointer.MayPrecede, unprime, unprime_heap, Pointer.toVar] at h
-      simp only [Nat.succ_eq_add_one, Fin.getElem_fin, Fin.coe_eq_castSucc, Fin.castSucc_lt_castSucc_iff] at h
-      simp only [Pointer.MayPrecede, unprime, unprime_heap, Pointer.toVar]
-      simp only [Nat.succ_eq_add_one, Fin.getElem_fin, Vector.getElem_map, Fin.coe_eq_castSucc, Fin.castSucc_lt_castSucc_iff]
-      simp only [unprime_node]
-      simp only [Fin.eta, Fin.mk_lt_mk, add_lt_add_iff_right, Fin.val_fin_lt]
-      refine Nat.sub_lt_sub_right ?_ h
-      simp only [Nat.succ_eq_add_one, Fin.coe_eq_castSucc, Pointer.toVar_node_eq, Fin.getElem_fin, Fin.castSucc_le_castSucc_iff] at hp
-      exact hp
-
-lemma unprime_relevantMayPrecede {B : Bdd n m} {x y : Pointer m} {hx : Pointer.Reachable (unprime p B).heap (unprime p B).root x} {hy : Pointer.Reachable (unprime p B).heap (unprime p B).root y} :
-    p ≤ x.toVar B.heap → B.RelevantMayPrecede ⟨x, unprime_reachable_iff.mpr hx⟩ ⟨y, unprime_reachable_iff.mpr hy⟩ → (unprime p B).RelevantMayPrecede ⟨x, hx⟩ ⟨y, hy⟩ := unprime_mayPrecede
-
-lemma unprime_relevantEdge {B : Bdd n m} {x y : Pointer m} {hx : Pointer.Reachable (unprime p B).heap (unprime p B).root x} {hy : Pointer.Reachable (unprime p B).heap (unprime p B).root y} :
-    (unprime p B).RelevantEdge ⟨x, hx⟩ ⟨y, hy⟩ → B.RelevantEdge ⟨x, unprime_reachable_iff.mpr hx⟩ ⟨y, unprime_reachable_iff.mpr hy⟩ := by
-  intro h
-  simp_all only [Bdd.RelevantEdge, unprime, unprime_heap]
-  cases h with
-  | low _ =>
-    left
-    simp_all [unprime_node]
-    assumption
-  | high _ =>
-    right
-    simp_all [unprime_node]
-    assumption
-
-lemma unprime_preserves_ordered {B : Bdd n m} {p : Fin n} : p ≤ B.var → Bdd.Ordered B → Bdd.Ordered (unprime p B) := by
-  intro hp ho
-  rintro ⟨x, hx⟩ _ hxy
-  apply unprime_relevantMayPrecede
-  · simp only [Nat.succ_eq_add_one, Fin.coe_eq_castSucc, Bdd.var] at hp
-    simp only [Nat.succ_eq_add_one, Fin.coe_eq_castSucc]
-    trans Pointer.toVar B.heap B.root
-    exact hp
-    apply Pointer.mayPrecede_of_reachable ho (unprime_reachable_iff.mpr hx)
-  · apply ho
-    exact unprime_relevantEdge hxy
-
-def ounprime (p : Fin n) (O : OBdd n m) : p ≤ O.1.var → OBdd (n - p) m
-  | hp => ⟨unprime p O.1, unprime_preserves_ordered hp O.2⟩
-
-lemma ounprime_low {O : OBdd n m} {h : O.1.root = .node j} {p: Fin n} {hp : p ≤ O.1.var} :
-    (OBdd.low (ounprime p O hp) h) = ounprime p (O.low h) (by trans O.1.var; exact hp; apply le_of_lt OBdd.var_lt_low_var) := by
-  rcases O with ⟨B, o⟩
-  simp only [OBdd.low]
-  congr
-  simp only [ounprime, unprime, unprime_heap, Bdd.low_heap_eq_heap]
-  simp only at h
-  simp_rw [h]
-  simp only [Bdd.low]
-  congr 1
-  simp_all only [Fin.getElem_fin, Vector.getElem_map]
-  rfl
-
-lemma ounprime_high {O : OBdd n m} {h : O.1.root = .node j} {p: Fin n} {hp : p ≤ O.1.var} :
-    (OBdd.high (ounprime p O hp) h) = ounprime p (O.high h) (by trans O.1.var; exact hp; apply le_of_lt OBdd.var_lt_high_var) := by
-  rcases O with ⟨B, o⟩
-  simp only [OBdd.high]
-  congr
-  simp only [ounprime, unprime, unprime_heap, Bdd.high_heap_eq_heap]
-  simp only at h
-  simp_rw [h]
-  simp only [Bdd.high]
-  congr 1
-  simp_all only [Fin.getElem_fin, Vector.getElem_map]
-  rfl
-
-lemma bunprime_low {n m j} {B : Bdd n m} {o : Bdd.Ordered B} {h : B.root = .node j} {p: Fin n} {hp : p ≤ B.var} :
-    (OBdd.low ⟨unprime p B, unprime_preserves_ordered hp o⟩ h) =
-    ⟨unprime p (OBdd.low ⟨B, o⟩ h).1,
-     unprime_preserves_ordered
-      (by trans B.var; exact hp; apply le_of_lt; rw [show B.var = (⟨B, o⟩ : OBdd n m).1.var by rfl]; apply OBdd.var_lt_low_var)
-      (OBdd.low ⟨B, o⟩ h).2⟩ := by
-  simp only [OBdd.low]
-  congr
-  simp only [unprime, unprime_heap, Bdd.low_heap_eq_heap]
-  simp_rw [h]
-  simp only [Bdd.low]
-  congr 1
-  simp_all only [Fin.getElem_fin, Vector.getElem_map]
-  rfl
-
-lemma bunprime_high {n m j} {B : Bdd n m} {o : Bdd.Ordered B} {h : B.root = .node j} {p: Fin n} {hp : p ≤ B.var} :
-    (OBdd.high ⟨unprime p B, unprime_preserves_ordered hp o⟩ h) =
-    ⟨unprime p (OBdd.high ⟨B, o⟩ h).1,
-     unprime_preserves_ordered
-      (by trans B.var; exact hp; apply le_of_lt; rw [show B.var = (⟨B, o⟩ : OBdd n m).1.var by rfl]; apply OBdd.var_lt_high_var)
-      (OBdd.high ⟨B, o⟩ h).2⟩ := by
-  simp only [OBdd.high]
-  congr
-  simp only [unprime, unprime_heap, Bdd.high_heap_eq_heap]
-  simp_rw [h]
-  simp only [Bdd.high]
-  congr 1
-  simp_all only [Fin.getElem_fin, Vector.getElem_map]
-  rfl
-
-theorem ounprime_evaluate (O : OBdd n m) {p : Fin n} (hp : p ≤ O.1.var) {I : Vector Bool (n - p)} {J : Vector Bool p} : OBdd.evaluate (ounprime p O hp) I = O.evaluate (Vector.cast (by omega) (J ++ I)) := by
-  simp only [ounprime]
-  cases O_root_def : O.1.root with
-  | terminal _ =>
-    simp only [unprime]
-    rw [OBdd.evaluate_terminal' O_root_def]
-    simp_rw [O_root_def]
-    rw [OBdd.evaluate_terminal]
-    simp
-  | node j =>
-    rw [OBdd.evaluate_node'' O_root_def]
-    have that : (⟨(unprime p O.1), unprime_preserves_ordered hp O.2⟩ : OBdd _ _).1.root = Pointer.node j := O_root_def
-    rw [OBdd.evaluate_node'' that]
-    simp only
-    congr 1
-    · simp only [eq_iff_iff, Bool.coe_iff_coe]
-      simp only [unprime, unprime_heap, Fin.getElem_fin, Vector.getElem_map, unprime_node]
-      simp only [Fin.eta]
-      rw [Vector.getElem_cast]
-      rw [Vector.getElem_append]
-      split
-      next contra =>
-        absurd contra
-        simp only [Nat.succ_eq_add_one, Fin.coe_eq_castSucc, Bdd.var] at hp
-        rw [O_root_def] at hp
-        simp at hp
-        omega
-      next => rfl
-    · have := ounprime_evaluate (O.high O_root_def) (I := I) (J := J)
-      rw [← this]
-      rw [← ounprime_high (hp := hp)]
-      rfl
-    · have := ounprime_evaluate (O.low O_root_def) (I := I) (J := J)
-      rw [← this]
-      rw [← ounprime_low (hp := hp)]
-      rfl
-termination_by O
-
-def tunprime (p : Fin n) (T : DecisionTree n) : T.lowerBoundedBy p → DecisionTree (n - p) := fun r ↦
-  match T with
-  | .leaf b => .leaf b
-  | .branch i l h => .branch ⟨i.1 - p, by omega⟩ (tunprime p l (DecisionTree.lowerBoundedBy_low r)) (tunprime p h (DecisionTree.lowerBoundedBy_high r))
-
-lemma tunprime_injective : tunprime x T1 h1 = tunprime x T2 h2 → T1 = T2 := by
+lemma trelabel_injective {f : Nat → Nat} {hf : ∀ i : Fin n, f i < f n} {h : ∀ i i' : Fin n, T1.usesVar i → T2.usesVar i' → f i = f i' → i = i'} :
+    trelabel hf T1 = trelabel hf T2 → T1 = T2 := by
   intro h
   cases T1 with
   | leaf _ =>
     cases T2 with
-    | leaf _ => simp only [tunprime] at h; simp_all
+    | leaf _ => simp only [trelabel] at h; simp_all
     | branch _ _ _ => contradiction
-  | branch v1 l1 r1 =>
+  | branch i tl th =>
     cases T2 with
     | leaf _ => contradiction
-    | branch v2 l2 r2 =>
-      simp only [tunprime] at h
+    | branch i' tl' th' =>
+      simp only [trelabel] at h
       injection h with a b c
-      rw [tunprime_injective b, tunprime_injective c]
+      rw [trelabel_injective b (hf := hf) (f := f)]
+      rw [trelabel_injective c (hf := hf) (f := f)]
       simp_all only [Fin.mk.injEq, DecisionTree.branch.injEq, and_self, and_true]
-      have : x.1 ≤ v1.1 := by
-        cases h1 with
-        | node _ _ _ => assumption
-      have : x.1 ≤ v2.1 := by
-        cases h2 with
-        | node _ _ _ => assumption
-      omega
+      apply h
+      · exact .here
+      · exact .here
+      · exact a
+      · intro ii ii' hii hii' hfi
+        apply h _ _ (DecisionTree.usesVar.high hii) (DecisionTree.usesVar.high hii') hfi
+      · intro ii ii' hii hii' hfi
+        apply h _ _ (DecisionTree.usesVar.low hii) (DecisionTree.usesVar.low hii') hfi
 
-lemma unprime_low {O : OBdd n m} {h : O.1.root = .node j} {p : Fin n} {hp : p ≤ O.1.var} :
-   (OBdd.low ⟨unprime p O.1, unprime_preserves_ordered hp O.2⟩ h) = ⟨unprime p (O.low h).1, unprime_preserves_ordered (by trans O.1.var; exact hp; apply le_of_lt; apply OBdd.var_lt_low_var) (O.low h).2⟩ := by
-  simp only [OBdd.low]
-  congr
-  simp only [unprime, unprime_heap, Bdd.low_heap_eq_heap]
-  simp_rw [h]
-  simp only [Bdd.low]
-  congr 1
-  simp_all only [Fin.getElem_fin, Vector.getElem_map]
-  rfl
-
-lemma unprime_high {O : OBdd n m} {h : O.1.root = .node j} {p : Fin n} {hp : p ≤ O.1.var} :
-   (OBdd.high ⟨unprime p O.1, unprime_preserves_ordered hp O.2⟩ h) = ⟨unprime p (O.high h).1, unprime_preserves_ordered (by trans O.1.var; exact hp; apply le_of_lt; apply OBdd.var_lt_high_var) (O.high h).2⟩ := by
-  simp only [OBdd.high]
-  congr
-  simp only [unprime, unprime_heap, Bdd.high_heap_eq_heap]
-  simp_rw [h]
-  simp only [Bdd.high]
-  congr 1
-  simp_all only [Fin.getElem_fin, Vector.getElem_map]
-  rfl
-
-lemma unprime_toTree_tunprime' {O : OBdd n m} {p : Fin n} {hp : p ≤ O.1.var} :
-    OBdd.toTree ⟨unprime p O.1, unprime_preserves_ordered hp O.2⟩ = tunprime p (OBdd.toTree O) (OBdd.toTree_lowerBoundedBy_var hp) := by
+lemma relabel_toTree_trelabel (O : OBdd n m) {f : Nat → Nat} (hf : ∀ i : Fin n, f i < f n)
+    (hu : ∀ i i' : Fin n, i < i' → O.1.usesVar i → O.1.usesVar i' → f i < f i') :
+    OBdd.toTree (orelabel O hf hu) = trelabel hf (OBdd.toTree O) := by
+  simp only [orelabel]
   cases O_root_def : O.1.root with
   | terminal _ =>
-    simp only [unprime]
-    simp_rw [OBdd.toTree_terminal' O_root_def]
+    simp only [relabel]
+    rw [OBdd.toTree_terminal' O_root_def]
     simp_rw [O_root_def]
     rw [OBdd.toTree_terminal]
-    simp [tunprime]
+    simp [trelabel]
   | node _ =>
-    simp_rw [OBdd.toTree_node O_root_def]
+    rw [OBdd.toTree_node O_root_def]
     rw [OBdd.toTree_node (by trans O.1.root; rfl; exact O_root_def)]
     simp only [Fin.getElem_fin]
     congr 1
-    · simp only [unprime, unprime_heap, Vector.getElem_map, unprime_node, Fin.eta, Bdd.Ordered.eq_1, Fin.mk.injEq, Nat.add_right_cancel_iff]
+    · simp only [relabel, relabel_heap, Vector.getElem_map, relabel_node, Fin.eta, Bdd.Ordered.eq_1, Fin.mk.injEq, Nat.add_right_cancel_iff]
       rfl
-    · have := unprime_toTree_tunprime' (O := (O.low O_root_def)) (p := p) (hp := (by trans O.1.var; exact hp; apply le_of_lt OBdd.var_lt_low_var))
-      rw [← unprime_low (hp := hp)] at this
+    · have := relabel_toTree_trelabel (O := (O.low O_root_def)) hf (fun i i' hii' hi hi' ↦ hu i i' hii' (OBdd.usesVar_of_low_usesVar hi) (OBdd.usesVar_of_low_usesVar hi'))
+      rw [← orelabel_low] at this
       exact this
-    · have := unprime_toTree_tunprime' (O := (O.high O_root_def)) (p := p) (hp := (by trans O.1.var; exact hp; apply le_of_lt OBdd.var_lt_high_var))
-      rw [← unprime_high (hp := hp)] at this
+    · have := relabel_toTree_trelabel (O := (O.high O_root_def)) hf (fun i i' hii' hi hi' ↦ hu i i' hii' (OBdd.usesVar_of_high_usesVar hi) (OBdd.usesVar_of_high_usesVar hi'))
+      rw [← orelabel_high] at this
       exact this
 termination_by O
 
-lemma unprime_toTree_tunprime {B : Bdd n m} {o : B.Ordered} {p : Fin n} {hp : p ≤ B.var} :
-    OBdd.toTree ⟨unprime p B, unprime_preserves_ordered hp o⟩ = tunprime p (OBdd.toTree ⟨B, o⟩) (OBdd.toTree_lowerBoundedBy_var hp) := by
-  let O : OBdd n m := ⟨B, o⟩
-  have : B = O.1 := rfl
-  simp_rw [this]
-  exact unprime_toTree_tunprime' (hp := hp)
+lemma relabel_toTree_trelabel' {B : Bdd n m} {o : B.Ordered} {f : Nat → Nat} (hf : ∀ i : Fin n, f i < f n)
+    (hu : ∀ i i' : Fin n, i < i' → B.usesVar i → B.usesVar i' → f i < f i') :
+    OBdd.toTree ⟨relabel hf B, relabel_preserves_ordered hu o⟩ = trelabel hf (OBdd.toTree ⟨B, o⟩) := relabel_toTree_trelabel ⟨B, o⟩ hf hu
 
-lemma unprime_preserves_noRedundancy {B : Bdd n m} : B.NoRedundancy → (unprime p B).NoRedundancy := by
-  rintro hnr ⟨p, hp⟩ contra
-  simp only at contra
-  cases p_def : p with
-  | terminal _ =>
-    cases contra with
-    | red _ => contradiction
-  | node j =>
-    rw [p_def] at contra
-    cases contra with
-    | red red =>
-      simp only [unprime, unprime_heap, Fin.getElem_fin, unprime_node] at red
-      apply hnr ⟨p, unprime_reachable_iff.mpr hp⟩
-      simp_rw [p_def]
-      constructor
-      simp_all only [Vector.getElem_map, Fin.getElem_fin]
-      simp only [unprime, unprime_heap, Fin.getElem_fin, unprime_node] at red
-      exact red
-
-lemma ounprime_preserves_similarRP {O : OBdd n m} {p q : Pointer m} {hx}
-    {hp : Pointer.Reachable (ounprime x O hx).1.heap (ounprime x O hx).1.root p} {hq : Pointer.Reachable (ounprime x O hx).1.heap (ounprime x O hx).1.root q} :
-    (ounprime x O hx).SimilarRP ⟨p, hp⟩ ⟨q, hq⟩ → O.SimilarRP ⟨p, unprime_reachable_iff.mpr hp⟩ ⟨q, unprime_reachable_iff.mpr hq⟩ := by
+lemma orelabel_preserves_similarRP {O : OBdd n m} {f : Nat → Nat} {hf : ∀ i : Fin n, f i < f n}
+    {hu : ∀ i i' : Fin n, i < i' → O.1.usesVar i → O.1.usesVar i' → f i < f i'}
+    {p q : Pointer m}
+    {hp : Pointer.Reachable (orelabel O hf hu).1.heap (orelabel O hf hu).1.root p}
+    {hq : Pointer.Reachable (orelabel O hf hu).1.heap (orelabel O hf hu).1.root q} :
+    (orelabel O hf hu).SimilarRP ⟨p, hp⟩ ⟨q, hq⟩ → O.SimilarRP ⟨p, relabel_reachable_iff.mpr hp⟩ ⟨q, relabel_reachable_iff.mpr hq⟩ := by
   intro sim
   simp only [OBdd.SimilarRP, OBdd.Similar, OBdd.HSimilar] at sim
   simp only [OBdd.SimilarRP, OBdd.Similar, OBdd.HSimilar]
@@ -682,151 +291,205 @@ lemma ounprime_preserves_similarRP {O : OBdd n m} {p q : Pointer m} {hx}
         rw [OBdd.toTree_node rfl]
       injection sim with ha hb hc
       simp only [Fin.getElem_fin] at ha
-      simp only [ounprime, unprime, unprime_heap, Vector.getElem_map, unprime_node, Fin.eta, Fin.mk.injEq, Nat.add_right_cancel_iff] at ha
+      simp only [orelabel, relabel, relabel_heap, Vector.getElem_map, relabel_node, Fin.eta, Fin.mk.injEq, Nat.add_right_cancel_iff] at ha
       conv =>
         lhs
         rw [OBdd.toTree_node rfl]
       conv =>
         rhs
         rw [OBdd.toTree_node rfl]
-      have this : x ≤ O.1.heap[j].var := by
-        apply Fin.le_iff_val_le_val.mpr
-        trans O.1.var.1
-        · simp only [Nat.succ_eq_add_one, Fin.coe_eq_castSucc, Bdd.var] at hx
-          simp only [Nat.succ_eq_add_one, Bdd.var]
-          exact hx
-        · have := Pointer.mayPrecede_of_reachable O.2 (unprime_reachable_iff.mpr hp)
-          simp only [Nat.succ_eq_add_one, Pointer.toVar_node_eq, Fin.getElem_fin, Fin.coe_eq_castSucc] at this
-          simp only [Nat.succ_eq_add_one, Bdd.var, Fin.getElem_fin, ge_iff_le]
-          exact this
-      have that : x ≤ O.1.heap[i].var := by
-        apply Fin.le_iff_val_le_val.mpr
-        trans O.1.var.1
-        · simp only [Nat.succ_eq_add_one, Fin.coe_eq_castSucc, Bdd.var] at hx
-          simp only [Nat.succ_eq_add_one, Bdd.var]
-          exact hx
-        · have := Pointer.mayPrecede_of_reachable O.2 (unprime_reachable_iff.mpr hq)
-          simp only [Nat.succ_eq_add_one, Pointer.toVar_node_eq, Fin.getElem_fin, Fin.coe_eq_castSucc] at this
-          simp only [Nat.succ_eq_add_one, Bdd.var, Fin.getElem_fin, ge_iff_le]
-          exact this
+      have help1 : ∀ x, Bdd.usesVar { heap := O.1.heap, root := Pointer.node j } x → O.1.usesVar x := by
+          rintro x ⟨jj, h1, h2⟩
+          use jj
+          constructor
+          · trans Pointer.node j
+            · exact relabel_reachable_iff.mpr hp
+            · exact h1
+          · exact h2
+      have help2 : ∀ x, Bdd.usesVar { heap := O.1.heap, root := Pointer.node i } x → O.1.usesVar x := by
+          rintro x ⟨jj, h1, h2⟩
+          use jj
+          constructor
+          · trans Pointer.node i
+            · exact relabel_reachable_iff.mpr hq
+            · exact h1
+          · exact h2
       congr 1
       · simp only
-        simp_all only [Fin.getElem_fin]
-        suffices s : O.1.heap[j.1].var - x.1 = O.1.heap[i.1].var - x.1 by omega
-        exact ha
-      · simp only [ounprime] at hb
-        simp only [unprime] at hb
-        simp_rw [← unprime.eq_1] at hb
+        by_contra c
+        apply ne_iff_lt_or_gt.mp at c
+        cases c with
+        | inl h => exact (ne_iff_lt_or_gt.mpr (.inl (hu O.1.heap[j].var O.1.heap[i].var h ⟨j, relabel_reachable_iff.mpr hp, rfl⟩ ⟨i, relabel_reachable_iff.mpr hq, rfl⟩))) ha
+        | inr h => exact (ne_iff_lt_or_gt.mpr (.inr (hu O.1.heap[i].var O.1.heap[j].var h ⟨i, relabel_reachable_iff.mpr hq, rfl⟩ ⟨j, relabel_reachable_iff.mpr hp, rfl⟩))) ha
+      · simp only [orelabel] at hb
+        simp only [relabel] at hb
+        simp_rw [← relabel.eq_1] at hb
         conv at hb =>
           lhs
-          rw [bunprime_low (h := rfl) (hp := (by simp; exact this)) (o := Bdd.ordered_of_reachable (unprime_reachable_iff.mpr hp))]
+          rw [brelabel_low (h := rfl) (o := Bdd.ordered_of_reachable (relabel_reachable_iff.mpr hp)) hf (by simp_all)]
         conv at hb =>
           rhs
-          rw [bunprime_low (h := rfl) (hp := (by simp; exact that)) (o := Bdd.ordered_of_reachable (unprime_reachable_iff.mpr hq))]
+          rw [brelabel_low (h := rfl) (o := Bdd.ordered_of_reachable (relabel_reachable_iff.mpr hq)) hf (by simp_all)]
         simp only [OBdd.low] at hb
         simp only [OBdd.low]
-        have this : x ≤ Pointer.toVar O.1.heap O.1.heap[j].low := by
-          apply Fin.le_iff_val_le_val.mpr
-          trans O.1.var.1
-          · simp only [Nat.succ_eq_add_one, Fin.coe_eq_castSucc, Bdd.var] at hx
-            simp only [Nat.succ_eq_add_one, Bdd.var]
-            simp_all
-            exact hx
-          · have := Pointer.mayPrecede_of_reachable O.2 (unprime_reachable_iff.mpr hp)
-            simp only [Nat.succ_eq_add_one, Pointer.toVar_node_eq, Fin.getElem_fin, Fin.coe_eq_castSucc] at this
-            simp only [Nat.succ_eq_add_one, Bdd.var, Fin.getElem_fin, ge_iff_le]
-            simp_all
-            apply Pointer.mayPrecede_of_reachable O.2
-            trans .node j
-            exact (unprime_reachable_iff.mpr hp)
-            apply Bdd.reachable_of_edge
-            left
-            rfl
-        have that : x ≤ Pointer.toVar O.1.heap O.1.heap[i].low := by
-          apply Fin.le_iff_val_le_val.mpr
-          trans O.1.var.1
-          · simp only [Nat.succ_eq_add_one, Fin.coe_eq_castSucc, Bdd.var] at hx
-            simp only [Nat.succ_eq_add_one, Bdd.var]
-            simp_all
-            exact hx
-          · have := Pointer.mayPrecede_of_reachable O.2 (unprime_reachable_iff.mpr hq)
-            simp only [Nat.succ_eq_add_one, Pointer.toVar_node_eq, Fin.getElem_fin, Fin.coe_eq_castSucc] at this
-            simp only [Nat.succ_eq_add_one, Bdd.var, Fin.getElem_fin, ge_iff_le]
-            simp_all
-            apply Pointer.mayPrecede_of_reachable O.2
-            trans .node i
-            exact (unprime_reachable_iff.mpr hq)
-            apply Bdd.reachable_of_edge
-            left
-            rfl
+        have helplj : ∀ x, Bdd.usesVar (({ heap := O.1.heap, root := Pointer.node j } : Bdd n m).low rfl) x → O.1.usesVar x := by
+          rintro _ hx
+          apply help1
+          apply Bdd.usesVar_of_low_usesVar hx
+        have helpli : ∀ x, Bdd.usesVar (({ heap := O.1.heap, root := Pointer.node i } : Bdd n m).low rfl) x → O.1.usesVar x := by
+          rintro _ hx
+          apply help2
+          apply Bdd.usesVar_of_low_usesVar hx
         conv at hb =>
           lhs
-          rw [unprime_toTree_tunprime (o := (by apply Bdd.low_ordered; exact Bdd.ordered_of_reachable (unprime_reachable_iff.mpr hp)))
-                                      (hp := (by exact this))]
+          rw [relabel_toTree_trelabel' (o := (by apply Bdd.low_ordered; exact Bdd.ordered_of_reachable (relabel_reachable_iff.mpr hp))) hf (by simp_all)]
         conv at hb =>
           rhs
-          rw [unprime_toTree_tunprime (o := (by apply Bdd.low_ordered; exact Bdd.ordered_of_reachable (unprime_reachable_iff.mpr hq)))
-                                      (hp := (by exact that))]
-        rw [tunprime_injective hb]
-      · simp only [ounprime] at hc
-        simp only [unprime] at hc
-        simp_rw [← unprime.eq_1] at hc
+          rw [relabel_toTree_trelabel' (o := (by apply Bdd.low_ordered; exact Bdd.ordered_of_reachable (relabel_reachable_iff.mpr hq))) hf (by simp_all)]
+        rw [trelabel_injective hb]
+        intro ii ii' hii hii' hfi
+        rw [← OBdd.toTree_usesVar] at hii hii'
+        contrapose hfi
+        apply ne_iff_lt_or_gt.mpr
+        cases ne_iff_lt_or_gt.mp hfi with
+        | inl hfi =>
+          left
+          apply hu
+          · exact hfi
+          · apply help1
+            apply Bdd.usesVar_of_low_usesVar
+            exact hii
+            rfl
+          · apply help2
+            apply Bdd.usesVar_of_low_usesVar
+            exact hii'
+            rfl
+        | inr hfi =>
+          right
+          apply hu
+          · exact hfi
+          · apply help2
+            apply Bdd.usesVar_of_low_usesVar
+            exact hii'
+            rfl
+          · apply help1
+            apply Bdd.usesVar_of_low_usesVar
+            exact hii
+            rfl
+      · simp only [orelabel] at hc
+        simp only [relabel] at hc
+        simp_rw [← relabel.eq_1] at hc
         conv at hc =>
           lhs
-          rw [bunprime_high (h := rfl) (hp := (by simp; exact this)) (o := Bdd.ordered_of_reachable (unprime_reachable_iff.mpr hp))]
+          rw [brelabel_high (h := rfl) (o := Bdd.ordered_of_reachable (relabel_reachable_iff.mpr hp)) hf (by simp_all)]
         conv at hc =>
           rhs
-          rw [bunprime_high (h := rfl) (hp := (by simp; exact that)) (o := Bdd.ordered_of_reachable (unprime_reachable_iff.mpr hq))]
+          rw [brelabel_high (h := rfl) (o := Bdd.ordered_of_reachable (relabel_reachable_iff.mpr hq)) hf (by simp_all)]
         simp only [OBdd.high] at hc
         simp only [OBdd.high]
-        have this : x ≤ Pointer.toVar O.1.heap O.1.heap[j].high := by
-          apply Fin.le_iff_val_le_val.mpr
-          trans O.1.var.1
-          · simp only [Nat.succ_eq_add_one, Fin.coe_eq_castSucc, Bdd.var] at hx
-            simp only [Nat.succ_eq_add_one, Bdd.var]
-            simp_all
-            exact hx
-          · have := Pointer.mayPrecede_of_reachable O.2 (unprime_reachable_iff.mpr hp)
-            simp only [Nat.succ_eq_add_one, Pointer.toVar_node_eq, Fin.getElem_fin, Fin.coe_eq_castSucc] at this
-            simp only [Nat.succ_eq_add_one, Bdd.var, Fin.getElem_fin, ge_iff_le]
-            simp_all
-            apply Pointer.mayPrecede_of_reachable O.2
-            trans .node j
-            exact (unprime_reachable_iff.mpr hp)
-            apply Bdd.reachable_of_edge
-            right
-            rfl
-        have that : x ≤ Pointer.toVar O.1.heap O.1.heap[i].high := by
-          apply Fin.le_iff_val_le_val.mpr
-          trans O.1.var.1
-          · simp only [Nat.succ_eq_add_one, Fin.coe_eq_castSucc, Bdd.var] at hx
-            simp only [Nat.succ_eq_add_one, Bdd.var]
-            simp_all
-            exact hx
-          · have := Pointer.mayPrecede_of_reachable O.2 (unprime_reachable_iff.mpr hq)
-            simp only [Nat.succ_eq_add_one, Pointer.toVar_node_eq, Fin.getElem_fin, Fin.coe_eq_castSucc] at this
-            simp only [Nat.succ_eq_add_one, Bdd.var, Fin.getElem_fin, ge_iff_le]
-            simp_all
-            apply Pointer.mayPrecede_of_reachable O.2
-            trans .node i
-            exact (unprime_reachable_iff.mpr hq)
-            apply Bdd.reachable_of_edge
-            right
-            rfl
+        have helphj : ∀ x, Bdd.usesVar (({ heap := O.1.heap, root := Pointer.node j } : Bdd n m).high rfl) x → O.1.usesVar x := by
+          rintro _ hx
+          apply help1
+          apply Bdd.usesVar_of_high_usesVar hx
+        have helphi : ∀ x, Bdd.usesVar (({ heap := O.1.heap, root := Pointer.node i } : Bdd n m).high rfl) x → O.1.usesVar x := by
+          rintro _ hx
+          apply help2
+          apply Bdd.usesVar_of_high_usesVar hx
         conv at hc =>
           lhs
-          rw [unprime_toTree_tunprime (o := (by apply Bdd.high_ordered; exact Bdd.ordered_of_reachable (unprime_reachable_iff.mpr hp)))
-                                      (hp := (by exact this))]
+          rw [relabel_toTree_trelabel' (o := (by apply Bdd.high_ordered; exact Bdd.ordered_of_reachable (relabel_reachable_iff.mpr hp))) hf (by simp_all)]
         conv at hc =>
           rhs
-          rw [unprime_toTree_tunprime (o := (by apply Bdd.high_ordered; exact Bdd.ordered_of_reachable (unprime_reachable_iff.mpr hq)))
-                                      (hp := (by exact that))]
-        rw [tunprime_injective hc]
+          rw [relabel_toTree_trelabel' (o := (by apply Bdd.high_ordered; exact Bdd.ordered_of_reachable (relabel_reachable_iff.mpr hq))) hf (by simp_all)]
+        rw [trelabel_injective hc]
+        intro ii ii' hii hii' hfi
+        rw [← OBdd.toTree_usesVar] at hii hii'
+        contrapose hfi
+        apply ne_iff_lt_or_gt.mpr
+        cases ne_iff_lt_or_gt.mp hfi with
+        | inl hfi =>
+          left
+          apply hu
+          · exact hfi
+          · apply help1
+            apply Bdd.usesVar_of_high_usesVar
+            exact hii
+            rfl
+          · apply help2
+            apply Bdd.usesVar_of_high_usesVar
+            exact hii'
+            rfl
+        | inr hfi =>
+          right
+          apply hu
+          · exact hfi
+          · apply help2
+            apply Bdd.usesVar_of_high_usesVar
+            exact hii'
+            rfl
+          · apply help1
+            apply Bdd.usesVar_of_high_usesVar
+            exact hii
+            rfl
 
-lemma ounprime_reduced {O : OBdd n m} {p : Fin n} {hp : p ≤ O.1.var} : O.Reduced → (ounprime p O hp).Reduced := by
+lemma orelabel_reduced {O : OBdd n m} {f : Nat → Nat} {hf : ∀ i : Fin n, f i < f n}
+    {hu : ∀ i i' : Fin n, i < i' → O.1.usesVar i → O.1.usesVar i' → f i < f i'} :
+    O.Reduced → (orelabel O hf hu).Reduced := by
   rintro ⟨r1, r2⟩
   constructor
-  · exact unprime_preserves_noRedundancy r1
-  · rintro _ _ sim; exact r2 (ounprime_preserves_similarRP sim)
+  · exact relabel_preserves_noRedundancy r1
+  · rintro _ _ sim
+    exact r2 (orelabel_preserves_similarRP sim)
+
+@[simp]
+def oprime p (O : OBdd n m) : OBdd (n + p) m := orelabel O (f := (· + p)) (by simp) (fun _ _ _ _ _ ↦ by simpa)
+
+theorem oprime_evaluate (O : OBdd n m) :
+    OBdd.evaluate (oprime p O) I = O.evaluate (Vector.cast (Eq.symm (Nat.eq_sub_of_add_eq rfl)) (I.drop p)) := by
+  simp only [oprime, orelabel_evaluate, Vector.drop_eq_cast_extract, Vector.cast_cast]
+  congr
+  ext i hi
+  simp only [Vector.getElem_ofFn, Vector.getElem_cast, Vector.getElem_extract]
+  simp_rw [add_comm]
+
+lemma oprime_reduced {O : OBdd n m} : O.Reduced → (oprime p O).Reduced := orelabel_reduced
+
+@[simp]
+def ounprime (p : Fin n) (O : OBdd n m) (hp : p ≤ O.1.var) : OBdd (n - p) m := orelabel O (f := (· - p)) (fun _ ↦ by simp_all; omega) (by
+  intro x y hxy hx hy
+  simp only
+  rcases p with ⟨pp, hp⟩
+  have : O.1.var.1 ≤ x.1 := by
+    rcases hx with ⟨jj, h1, h2⟩
+    rw [← h2]
+    rw [show O.1.heap[jj].var.1 = Pointer.toVar O.1.heap (Pointer.node jj) by simp]
+    apply Pointer.mayPrecede_of_reachable O.2 h1
+  simp_all only [Nat.succ_eq_add_one, gt_iff_lt]
+  refine Nat.sub_lt_sub_right ?_ hxy
+  trans O.1.var.1
+  rw [Fin.le_iff_val_le_val] at hp
+  simp_all only [Fin.val_natCast, Nat.succ_eq_add_one]
+  rw [show pp % (n + 1) = pp from (Nat.mod_eq_of_lt (by omega))] at hp
+  repeat assumption)
+
+theorem ounprime_evaluate (O : OBdd n m) {p : Fin n} (hp : p ≤ O.1.var) {I : Vector Bool (n - p)} {J : Vector Bool p} :
+    OBdd.evaluate (ounprime p O hp) I = O.evaluate (Vector.cast (by omega) (J ++ I)) := by
+  simp only [ounprime, orelabel_evaluate]
+  apply OBdd.evaluate_eq_of_forall_usesVar
+  intro i hi
+  simp only [Fin.getElem_fin, Vector.getElem_ofFn, Vector.getElem_cast]
+  have : O.1.var.1 ≤ i.1 := by
+    rcases hi with ⟨jj, h1, h2⟩
+    rw [← h2]
+    rw [show O.1.heap[jj].var.1 = Pointer.toVar O.1.heap (Pointer.node jj) by simp]
+    apply Pointer.mayPrecede_of_reachable O.2 h1
+  have : p.1 ≤ i.1 := by
+    rw [Fin.le_iff_val_le_val] at hp
+    simp_all only [Nat.succ_eq_add_one, Fin.coe_eq_castSucc, Fin.coe_castSucc, Fin.val_fin_le]
+    omega
+  rw [Vector.getElem_append_right]
+  exact this
+
+lemma ounprime_reduced {O : OBdd n m} {p : Fin n} {hp : p ≤ O.1.var} : O.Reduced → (ounprime p O hp).Reduced := orelabel_reduced
 
 end Prime
